protocols/GenProtoSS.v
@@ -127,9 +127,6 @@ Module MyProtocolSecure <: AutomatedSafeProtocolSS.
 
   Qed.
 
-  (* Show Ltac Profile. *)
-  (* Show Ltac Profile "churn2". *)
-  
   Lemma U_good : @universe_starts_sane _ Unit b ru0.
   Proof.
     autounfold;
@@ -138,9 +135,8 @@ Module MyProtocolSecure <: AutomatedSafeProtocolSS.
     - solve_perm_merges; eauto.
     - econstructor.
     - unfold AdversarySafety.keys_honest; rewrite Forall_natmap_forall; intros.
-      econstructor; unfold mkrUsr; simpl.
+      unfold mkrUsr; simpl.
       rewrite !findUserKeys_add_reduce, findUserKeys_empty_is_empty; eauto.
-      solve_perm_merges.
     - unfold lameAdv; simpl; eauto.
   Qed.
   
